theories/Ast.v
@@ -2,7 +2,7 @@ Require Import Coq.Strings.String.
 Require Import Coq.PArith.BinPos.
 Require Import List. Import ListNotations.
 From Template Require Import monad_utils.
-From Template Require Export univ.
+From Template Require Export univ uGraph.
 
 Definition ident := string. (* e.g. nat *)
 Definition kername := string. (* e.g. Coq.Init.Datatypes.nat *)
